add the version with concurrency

theories/heap_lang_examples/very_awkward.v
@@ -15,6 +15,20 @@ Definition very_awkward_self_apply : expr :=
   let: "f" := very_awkward in
   "f" (λ: <>, "f" (λ: <>, #());; #()).
 
+Definition factorial : val :=
+  rec: "fact" "n" := if: "n" = #0 then #1 else "n" * ("fact" ("n" - #1)).
+
+Definition call_fact_across : expr :=
+  let: "b" := ref #true in
+  let: "c" := ref NONE in
+  let: "wait" := rec: "w" <> := if: ! "c" = NONE then "w" #() else #() in
+  λ: <>, if: ! "b" then "b"  <- #false;; Fork (factorial #1000000) else "wait" #().
+
+Definition very_akward_call_fact_across : expr :=
+  let: "g" := call_fact_across in
+  let: "h" := very_awkward in
+  "h" "g".
+
 Section very_awkward.
   Context `{!wbheapGS Σ} `{!oneshotG Σ}.
 
@@ -118,6 +132,94 @@ Section very_awkward.
     iApply "HΨ"; done.
   Qed.
 
+  (* a very weak spec just showing safety of factorial *)
+  Lemma wp_factorial (n : Z) :
+    ⊢ {{{ True }}} factorial #n {{{ (k : Z), RET #k; True }}}.
+  Proof.
+    rewrite /factorial.
+    iLöb as "IH" forall (n).
+    iIntros "!#" (Φ) "_ HΦ".
+    wp_pures.
+    destruct (decide (n = 0)) as [->|].
+    - wp_pures. iApply "HΦ"; done.
+    - rewrite bool_decide_eq_false_2; last by intros ?; simplify_eq.
+      do 2 wp_pure.
+      wp_apply "IH"; first done.
+      iIntros (k) "_"; wp_pures.
+      iModIntro.
+      iApply "HΦ"; done.
+  Qed.
+
+  Lemma wp_call_fact_across :
+    ⊢ {{{ True }}} call_fact_across {{{(f : val), RET f; {{{ True }}} f #() {{{ RET #(); True }}} }}}.
+  Proof.
+    iIntros "!#" (Φ) "_ HΦ".
+    rewrite /call_fact_across.
+    wp_alloc b as "Hb".
+    wp_pures.
+    wp_alloc c as "Hc".
+    wp_pures.
+    iMod (inv_alloc (nroot .@ "cfa") _
+            (∃ (a : bool), b ↦ #a ∗ (c ↦ NONEV ∨ ∃ (n : nat), c ↦ SOMEV #n)) with "[Hb Hc]")
+      as "#Hinv".
+    { iExists _; iFrame. }
+    iModIntro.
+    iApply "HΦ".
+    clear Φ.
+    iIntros "!#" (Φ) "_ HΦ".
+    wp_pures.
+    wp_bind (! _)%E.
+    iInv (nroot .@ "cfa") as (a) "[Hb Hc]".
+    wp_load.
+    iModIntro.
+    iSplitL "Hb Hc"; first by iFrame "Hc"; eauto.
+    destruct a.
+    - wp_pures.
+      wp_bind (_ <- _)%E.
+      iInv (nroot .@ "cfa") as (a) "[Hb Hc]".
+      wp_store.
+      iModIntro.
+      iSplitL "Hb Hc"; first by iFrame "Hc"; eauto.
+      wp_pures.
+      iApply wp_fork.
+      + iNext; iApply wp_factorial; done.
+      + iNext; iApply "HΦ"; done.
+    - wp_pure.
+      iLöb as "IH".
+      wp_pures.
+      wp_bind (! _)%E.
+      iInv (nroot .@ "cfa") as (a) "[Hb [Hc|Hc]]".
+      + wp_load.
+        iModIntro.
+        iSplitL "Hb Hc"; first by iExists _; iFrame.
+        do 2 wp_pure.
+        iApply "IH"; done.
+      + iDestruct "Hc" as (?) "Hc".
+        wp_load.
+        iModIntro.
+        iSplitL "Hb Hc"; first by iExists _; iFrame; eauto.
+        wp_pures. iApply "HΦ"; done.
+  Qed.
+
+  Lemma wbwp_very_akward_call_fact_across :
+    ⊢ WBWP very_akward_call_fact_across {{v, ⌜v = #1⌝ }}.
+  Proof.
+    rewrite /very_akward_call_fact_across.
+    wbwp_bind call_fact_across.
+    iApply wp_wbwp.
+    iApply wp_call_fact_across; first done.
+    iNext.
+    iIntros (g) "#Hg".
+    wbwp_pures.
+    wbwp_apply wbwp_very_awkward; first done.
+    iIntros (h) "#Hh".
+    wbwp_pures.
+    iApply "Hh"; last done.
+    iIntros "!#" (Φ) "_ HΦ".
+    iApply wp_wbwp.
+    iApply "Hg"; done.
+  Qed.
+
 End very_awkward.
 
 Theorem very_awkward_self_apply_returns_one σ :
@@ -126,4 +228,12 @@ Proof.
   set (Σ := #[heapΣ; oneshotΣ]).
   apply (wbheap_adequacy Σ).
   iIntros (?) "?". iApply wbwp_very_awkward_self_apply.
+Qed.
+
+Theorem wbwp_very_akward_call_fact_across_returns_one σ :
+  adequate NotStuck very_akward_call_fact_across σ (λ v _, v = #1).
+Proof.
+  set (Σ := #[heapΣ; oneshotΣ]).
+  apply (wbheap_adequacy Σ).
+  iIntros (?) "?". iApply wbwp_very_akward_call_fact_across.
 Qed.
