theories/heap_lang_trace_examples/very_awkward.v
@@ -1,5 +1,6 @@
 From iris.algebra Require Import agree.
 From iris.base_logic Require Import invariants.
+From WBLogrel Require Import oneshot.
 From WBLogrel.heap_lang_trace Require Import adequacy notation proofmode.
 
 (** ** Proof that the very awkward example specification guarantees
@@ -166,4 +167,255 @@ Proof.
   { iIntros (? ? ?) "!> Hφ". iApply Hinit; eauto. }
   { iIntros (?). iApply Wrap.correct. iApply Hlib. }
   eauto.
+Qed.
+
+(* concretizing with concrete programs. *)
+
+Definition very_awkward : expr :=
+  let: "l" := ref #0 in
+  λ: "f", "l" <- #0;; "f" #();; "l" <- #1;; "f" #();; ! "l".
+
+Definition very_awkward_self_apply very_awk : expr :=
+  let: "f" := very_awk in
+  "f" (λ: <>, "f" (λ: <>, #());; #()).
+
+
+Definition factorial : val :=
+  rec: "fact" "n" := if: "n" = #0 then #1 else "n" * ("fact" ("n" - #1)).
+
+Definition call_fact_across : expr :=
+  let: "b" := ref #true in
+  let: "c" := ref NONE in
+  let: "wait" := rec: "w" <> := if: ! "c" = NONE then "w" #() else #() in
+  λ: <>, if: ! "b" then "b"  <- #false;; Fork (factorial #1000000) else "wait" #().
+
+Definition very_akward_call_fact_across very_awk : expr :=
+  let: "h" := very_awk in
+  let: "g" := call_fact_across in
+  "h" "g".
+
+Section very_awkward.
+  Context `{!wbheapGS Σ} `{!oneshotG Σ}.
+
+  Lemma wbwp_very_awkward : ⊢ very_awk_spec True very_awkward.
+  Proof.
+    rewrite /very_awkward /very_awk_spec.
+    iIntros (Φ) "_ !# HΦ".
+    wbwp_alloc l as "Hl".
+    wbwp_pures.
+    iMod new_pending as (γ) "Hpen".
+    iApply (wbwp_make_gstack _ _ γ); iIntros (n) "Hfr".
+    iDestruct (gstack_frag_exists with "Hfr") as "#Hx".
+    iMod (inv_alloc
+            (nroot .@ "awk") _
+            (∃ γ s, gstack_frag n s ∗ ⌜gtop s = Some γ⌝ ∗
+               ((pending γ ∗ l ↦ #0) ∨ (shot γ ∗ l ↦ #1)))%I with "[Hpen Hfr Hl]") as "#Hinv".
+    { iNext; iExists γ, _. iFrame "Hfr". iSplit; first by rewrite gtop_gsingleton. iLeft; iFrame. }
+    iApply wbwp_value.
+    iApply "HΦ".
+    clear Φ.
+    iIntros (g) "!#".
+    iIntros (Φ) "#Hg HΦ".
+    wbwp_pures.
+    iApply (wbwp_get_gstack_full n with "[$]"); first done.
+    iIntros (s) "Hfl".
+    wbwp_bind (_ <- _)%E.
+    iInv (nroot .@ "awk") as (γ1 s') ">(Hfr & % & Hl)" "Hcl".
+    iAssert (∃ v, l ↦ v ∗ (pending γ1 ∨ shot γ1))%I with "[Hl]" as (?) "[Hl Hps]".
+    { iDestruct "Hl" as "[[? ?]|[? ?]]"; iExists _; iFrame. }
+    iDestruct (gstacks_agree with "Hfl Hfr") as %<-.
+    iMod (new_pending) as (γ2) "Hpen2".
+    iMod (gstack_push _ _ _ γ2 with "Hfl Hfr") as "[Hfl Hfr]".
+    wbwp_store.
+    iApply wbwp_value.
+    iMod ("Hcl" with "[Hpen2 Hfr Hl]") as "_".
+    { iNext; iExists γ2, _; iFrame "Hfr"; iSplit; first by rewrite gtop_gpush. iLeft; iFrame. }
+    iModIntro.
+    wbwp_pures.
+    iAssert (|==> shot γ1)%I with "[Hps]" as ">#Hsh".
+    { iDestruct "Hps" as "[Hp|Hs]"; last done. iApply shoot; done. }
+    wbwp_bind (g _)%E.
+    iApply (wbwp_wand with "[Hfl]").
+    { iApply (wbwp_mend with "Hfl").
+      replace ((∅ ∪ {[n]}) ∖ {[n]}) with (∅ : gset ghost_id) by set_solver.
+      iApply ("Hg" $! (λ w, ⌜w = #()⌝)%I); done. }
+    iIntros (?) "[Hfl ->] /=".
+    wbwp_pures.
+    wbwp_bind (_ <- _)%E.
+    iInv (nroot .@ "awk") as (γ3 s') ">(Hfr & % & Hl)" "Hcl".
+    iAssert (∃ v, l ↦ v)%I with "[Hl]" as (?) "Hl".
+    { iDestruct "Hl" as "[[? ?]|[? ?]]"; iExists _; iFrame. }
+    iDestruct (gstacks_agree with "Hfl Hfr") as %<-.
+    iMod (gstack_pop with "Hfl Hfr") as "[Hfl Hfr]".
+    wbwp_store.
+    iApply wbwp_value.
+    iMod ("Hcl" with "[Hfr Hl]") as "_".
+    { iNext; iExists γ1, _; iFrame "Hfr". iSplit; first done. iRight; iFrame; done. }
+    iModIntro. simpl.
+    wbwp_pures.
+    wbwp_bind (g _)%E.
+    iApply (wbwp_wand with "[Hfl]").
+    { iApply (wbwp_mend with "Hfl").
+      replace ((∅ ∪ {[n]}) ∖ {[n]}) with (∅ : gset ghost_id) by set_solver.
+      iApply ("Hg" $! (λ w, ⌜w = #()⌝)%I); done. }
+    iIntros (?) "[Hfl ->]"; simplify_eq/=.
+    wbwp_pures.
+    iInv (nroot .@ "awk") as (γ4 s') ">(Hfr & % & Hl)" "Hcl".
+    iDestruct (gstacks_agree with "Hfl Hfr") as %<-.
+    simplify_eq.
+    iDestruct "Hl" as "[[Hp _]|[_ Hl]]".
+    { iExFalso; iApply shot_not_pending; done. }
+    wbwp_load.
+    iApply wbwp_value.
+    iMod ("Hcl" with "[Hfr Hl]") as "_".
+    { iNext; iExists _, _; iFrame. iSplit; first done. iRight; iFrame; done. }
+    iModIntro.
+    iFrame. iApply "HΦ"; done.
+  Qed.
+
+  Lemma wbwp_very_awkward_self_apply P very_awk :
+    very_awk_spec P very_awk -∗ {WB{{ P }}} very_awkward_self_apply very_awk {{{ RET #1; True }}}.
+  Proof.
+    rewrite /very_awkward_self_apply.
+    iIntros "#Hawk !#" (Φ) "HP HΦ".
+    wbwp_apply ("Hawk" with "[$]").
+    iIntros (f) "#Hf".
+    wbwp_pures.
+    wbwp_apply "Hf"; last done.
+    clear Φ.
+    iIntros "!#" (Φ) "_ HΦ".
+    wbwp_pures.
+    wbwp_apply "Hf"; last first.
+    { iIntros; wbwp_pures; iApply wbwp_value; iApply "HΦ"; done. }
+    iIntros "!#" (Ψ) "_ HΨ".
+    wbwp_pures.
+    iApply wbwp_value.
+    iApply "HΨ"; done.
+  Qed.
+
+  (* a very weak spec just showing safety of factorial *)
+  Lemma wp_factorial (n : Z) :
+    ⊢ {{{ True }}} factorial #n {{{ (k : Z), RET #k; True }}}.
+  Proof.
+    rewrite /factorial.
+    iLöb as "IH" forall (n).
+    iIntros "!#" (Φ) "_ HΦ".
+    wp_pures.
+    destruct (decide (n = 0)) as [->|].
+    - wp_pures. iApply "HΦ"; done.
+    - rewrite bool_decide_eq_false_2; last by intros ?; simplify_eq.
+      do 2 wp_pure.
+      wp_apply "IH"; first done.
+      iIntros (k) "_"; wp_pures.
+      iModIntro.
+      iApply "HΦ"; done.
+  Qed.
+
+  Lemma wp_call_fact_across :
+    ⊢ {{{ True }}} call_fact_across {{{(f : val), RET f; {{{ True }}} f #() {{{ RET #(); True }}} }}}.
+  Proof.
+    iIntros "!#" (Φ) "_ HΦ".
+    rewrite /call_fact_across.
+    wp_alloc b as "Hb".
+    wp_pures.
+    wp_alloc c as "Hc".
+    wp_pures.
+    iMod (inv_alloc (nroot .@ "cfa") _
+            (∃ (a : bool), b ↦ #a ∗ (c ↦ NONEV ∨ ∃ (n : nat), c ↦ SOMEV #n)) with "[Hb Hc]")
+      as "#Hinv".
+    { iExists _; iFrame. }
+    iModIntro.
+    iApply "HΦ".
+    clear Φ.
+    iIntros "!#" (Φ) "_ HΦ".
+    wp_pures.
+    wp_bind (! _)%E.
+    iInv (nroot .@ "cfa") as (a) "[Hb Hc]".
+    wp_load.
+    iModIntro.
+    iSplitL "Hb Hc"; first by iFrame "Hc"; eauto.
+    destruct a.
+    - wp_pures.
+      wp_bind (_ <- _)%E.
+      iInv (nroot .@ "cfa") as (a) "[Hb Hc]".
+      wp_store.
+      iModIntro.
+      iSplitL "Hb Hc"; first by iFrame "Hc"; eauto.
+      wp_pures.
+      iApply wp_fork.
+      + iNext; iApply wp_factorial; done.
+      + iNext; iApply "HΦ"; done.
+    - wp_pure.
+      iLöb as "IH".
+      wp_pures.
+      wp_bind (! _)%E.
+      iInv (nroot .@ "cfa") as (a) "[Hb [Hc|Hc]]".
+      + wp_load.
+        iModIntro.
+        iSplitL "Hb Hc"; first by iExists _; iFrame.
+        do 2 wp_pure.
+        iApply "IH"; done.
+      + iDestruct "Hc" as (?) "Hc".
+        wp_load.
+        iModIntro.
+        iSplitL "Hb Hc"; first by iExists _; iFrame; eauto.
+        wp_pures. iApply "HΦ"; done.
+  Qed.
+
+  Lemma wbwp_very_akward_call_fact_across P very_awk :
+    very_awk_spec P very_awk -∗
+    {WB{{ P }}} very_akward_call_fact_across very_awk {{{ RET #1; True }}}.
+  Proof.
+    rewrite /very_akward_call_fact_across /very_awk_spec.
+    iIntros "#Hawk !#" (Φ) "HP HΦ".
+    wbwp_apply ("Hawk" with "[$]").
+    iIntros (h) "#Hh".
+    wbwp_pures.
+    wbwp_bind call_fact_across.
+    iApply wp_wbwp.
+    iApply wp_call_fact_across; first done.
+    iNext.
+    iIntros (g) "#Hg".
+    wbwp_pures.
+    iApply "Hh"; last done.
+    clear Φ.
+    iIntros "!#" (Φ) "_ HΦ".
+    iApply wp_wbwp.
+    iApply "Hg"; done.
+  Qed.
+
+End very_awkward.
+
+Theorem very_awkward_self_apply_returns_one :
+    ∀ σ' e',
+      rtc erased_step ([((#();; #());; very_awkward_self_apply (Wrap.very_awk_instrumented very_awkward))%E], empty_state)
+        (e', σ') →
+      sequential_trace (trace σ').
+Proof.
+  assert (∀ Σ, subG (GFunctor (agreeR (leibnizO (list val)))) Σ → inG Σ (agreeR (leibnizO (list val)))).
+  { solve_inG. }
+  set (Σ := #[heapΣ; oneshotΣ; GFunctor (agreeR (leibnizO (list val)))]).
+  apply (@wrap_very_awk_correct Σ _ _ _ _ _ True%I).
+  - iIntros (?) "!#"; iIntros (?) "_ H"; wp_pures; iApply "H"; done.
+  - intros; apply wbwp_very_awkward.
+  - iIntros (? ? ?) "#? !#"; iIntros (?) "HP H".
+    iApply (wbwp_very_awkward_self_apply with "[$] [$]").
+    iNext; iIntros "_"; iApply "H"; done.
+Qed.
+
+Theorem wbwp_very_akward_call_fact_across_returns_one :
+    ∀ σ' e',
+      rtc erased_step ([((#();; #());; very_akward_call_fact_across (Wrap.very_awk_instrumented very_awkward))%E], empty_state)
+        (e', σ') →
+      sequential_trace (trace σ').
+Proof.
+  assert (∀ Σ, subG (GFunctor (agreeR (leibnizO (list val)))) Σ → inG Σ (agreeR (leibnizO (list val)))).
+  { solve_inG. }
+  set (Σ := #[heapΣ; oneshotΣ; GFunctor (agreeR (leibnizO (list val)))]).
+  apply (@wrap_very_awk_correct Σ _ _ _ _ _ True%I).
+  - iIntros (?) "!#"; iIntros (?) "_ H"; wp_pures; iApply "H"; done.
+  - intros; apply wbwp_very_awkward.
+  - iIntros (? ? ?) "#? !#"; iIntros (?) "HP H".
+    iApply (wbwp_very_akward_call_fact_across with "[$] [$]").
+    iNext; iIntros "_"; iApply "H"; done.
 Qed.
